\documentclass{article}
\usepackage[utf8]{inputenc}

\title{Maths Solution}
\author{Anofiu Jelilat }
\date{September 2020}

\usepackage{natbib}
\usepackage{graphicx}
\usepackage{amsmath}
\begin{document}

\maketitle

\section*{Question}
(Please show your workings). Over all real numbers, find the minimum value of a positive real number, $y$ such that
$$y = \sqrt{((x+6)^2 + 25)}+ \sqrt{((x-6)^2 + 121)}$$

\section*{Solution}
Recall that $y$ is said to have a minimum value at the point $x$ where $y^{'}(x) = 0$.\\\\
Let $u = \sqrt{((x+6)^2 + 25)}$ and $v = \sqrt{((x-6)^2 + 121)}$. Hence, $y^{'} = u^{'} + v^{'}$.\\\\
Also let $u = \sqrt{a},$ where $a = (x+6)^2 + 25$. $u^{'} = \frac{du}{da}\times \frac{da}{dx}$\\\\
$u^{'} = -2(x+6)\times \frac{1}{2}a^{-\frac{1}{2}} $. Similarly, $v^{'} = -2(x-6)\times \frac{1}{2}b^{-\frac{1}{2}} $, where $b = (x-6)^2 + 121$. \\\\
$\implies y^{'} = \dfrac{(x+6)}{((x+6)^{2}+25)^{\frac{1}{2}}} + \dfrac{(x-6)}{((x-6)^{2}+121))^{\frac{1}{2}}} = 0$\\
$\implies (x+6)((x-6)^{2}+121))^{\frac{1}{2}} + (x-6)((x+6)^{2}+25)^{\frac{1}{2}} = 0$\\
$\implies (x+6)((x-6)^{2}+121))^{\frac{1}{2}} = -(x-6)((x+6)^{2}+25)^{\frac{1}{2}}$\\
$\implies (x+6)^{2}((x-6)^{2}+121)= (x-6)^{2}((x+6)^{2}+25)$\\
$\implies 121(x+6)^{2}=25(x-6)^{2}$\\
$\implies 11(x+6)=5(x-6)$\\
$\implies 11x+66-5x+30 \implies 6x = 96$\\
$\implies x = 16$\\\\
Hence, $y$ is at a minimum when $x = 16$. So, we have the minimum value of $y = \sqrt{((16+6)^2 + 25)}+ \sqrt{((16-6)^2 + 121)}=37.43$
\end{document}
